src/lowparse/LowParse.Endianness.BitFields.fst
@@ -1,0 +1,43 @@
+module LowParse.Endianness.BitFields
+include LowParse.Endianness
+module BF = LowParse.BitFields
+
+module S = FStar.Seq
+
+open FStar.Mul
+
+let slice_n_to_be_bitfield
+  (len: pos)
+  (n: nat)
+  (i j: nat)
+: Lemma
+  (requires (
+    i <= j /\
+    j <= len /\
+    n < pow2 (8 * len)
+  ))
+  (ensures (
+    S.slice (n_to_be len n) i j == n_to_be (j - i) (BF.get_bitfield #(8 * len) n (8 * (len - j)) (8 * (len - i)))
+  ))
+= slice_n_to_be len n i j;
+  BF.get_bitfield_eq #(8 * len) n (8 * (len - j)) (8 * (len - i))
+
+module U8 = FStar.UInt8
+
+let bitfield_be_to_n_slice
+  (s: S.seq U8.t)
+  (i: nat)
+  (j: nat)
+: Lemma
+  (requires (
+    Seq.length s > 0 /\
+    i <= j /\ j <= S.length s
+  ))
+  (ensures (
+    let len = S.length s in
+    be_to_n s < pow2 (8 * len) /\
+    be_to_n (S.slice s i j) == BF.get_bitfield #(8 * len) (be_to_n s) (8 * (len - j)) (8 * (len - i))
+  ))
+= let len = S.length s in
+  lemma_be_to_n_is_bounded s;
+  slice_n_to_be_bitfield len (be_to_n s) i j
